src/program_proof/simplefs/bytes_proof.v
@@ -1,0 +1,114 @@
+From Perennial.program_proof Require Import proof_prelude.
+From Perennial.program_proof Require Import disk_prelude.
+From Perennial.Helpers Require Import NatDivMod bytes.
+Import Nat.
+
+From Goose.github_com Require Import tchajed.simplefs.bitmap.
+
+From Perennial.program_proof.simplefs Require Import bitmap_byte.
+
+Set Default Proof Using "Type".
+
+#[local] Unset Printing Projections.
+#[local] Ltac Zify.zify_post_hook ::= Z.div_mod_to_equations.
+
+Section proof.
+Context `{!heapGS Σ}.
+
+Lemma inj_lit_byte (b1 b2: w8) :
+  #b1 = #b2 ↔ b1 = b2.
+Proof.
+  split; [ | congruence ].
+  inversion 1; auto.
+Qed.
+
+Lemma bool_decide_byte_val_eq (b1 b2: w8) :
+  bool_decide (#b1 = #b2) = bool_decide (b1 = b2).
+Proof.
+  apply bool_decide_ext.
+  rewrite inj_lit_byte //.
+Qed.
+
+Lemma bool_decide_byte_val_neq (b1 b2: w8) :
+  bool_decide (#b1 ≠ #b2) = bool_decide (b1 ≠ b2).
+Proof.
+  apply bool_decide_ext.
+  rewrite inj_lit_byte.
+  split; try congruence.
+Qed.
+
+Lemma getBit_pure (b: w8) (i: w64) :
+  uint.Z i < 8 →
+  byte_to_bits b !!! uint.nat i =
+  bool_decide (word.and b (word.slu (W8 1) (W8 (uint.Z i))) ≠ W8 0).
+Proof.
+  intros.
+  bit_off_cases (uint.Z i); byte_cases b; vm_compute; reflexivity.
+Qed.
+
+Theorem wp_getBit (b : w8) (i : u64) :
+  {{{ ⌜uint.Z i < 8⌝ }}}
+    getBit #b #i
+  {{{ RET #(LitBool $ byte_to_bits b !!! (uint.nat i)); True }}}.
+Proof.
+  (*@ func getBit(b byte, i uint64) bool {                                    @*)
+  (*@     return b&(1<<i) != 0                                                @*)
+  (*@ }                                                                       @*)
+  iIntros (Φ) "Hpre HΦ". iDestruct "Hpre" as "%".
+  wp_call. iModIntro.
+  iDestruct ("HΦ" with "[//]") as "HΦ".
+  iExactEq "HΦ".
+  repeat f_equal.
+  rewrite -bool_decide_not bool_decide_byte_val_neq.
+  rewrite getBit_pure //.
+Qed.
+
+Lemma setBit_pure (b: w8) (i: Z) :
+  0 ≤ i < 8 →
+  byte_to_bits (word.or b (word.slu (W8 1) (W8 i))) =
+  <[Z.to_nat i:=true]> (byte_to_bits b).
+Proof.
+  intros.
+  bit_off_cases i; byte_cases b; reflexivity.
+Qed.
+
+Theorem wp_setBit (b : w8) (i : u64) :
+  {{{ ⌜uint.Z i < 8⌝ }}}
+    setBit #b #i
+  {{{ (b': w8), RET #b'; ⌜byte_to_bits b' = <[ uint.nat i := true ]> (byte_to_bits b)⌝ }}}.
+Proof.
+  (*@ func setBit(b byte, i uint64) byte {                                    @*)
+  (*@     return b | 1<<i                                                     @*)
+  (*@ }                                                                       @*)
+  iIntros (Φ) "Hpre HΦ". iDestruct "Hpre" as "%".
+  wp_call. iModIntro.
+  iApply "HΦ".
+  iPureIntro.
+  rewrite setBit_pure //. word.
+Qed.
+
+Lemma clearBit_pure (b: w8) (i: Z) :
+  0 ≤ i < 8 →
+  byte_to_bits (word.and b (word.not (word.slu (W8 1) (W8 i)))) =
+  <[Z.to_nat i:=false]> (byte_to_bits b).
+Proof.
+  intros.
+  bit_off_cases i; byte_cases b; reflexivity.
+Qed.
+
+Theorem wp_clearBit (b : w8) (i : u64) :
+  {{{ ⌜uint.Z i < 8⌝ }}}
+    clearBit #b #i
+  {{{ (b': w8), RET #b'; ⌜byte_to_bits b' = <[ uint.nat i := false ]> (byte_to_bits b)⌝ }}}.
+Proof.
+  (*@ func clearBit(b byte, i uint64) byte {                                  @*)
+  (*@     return b & ^(1 << i)                                                @*)
+  (*@ }                                                                       @*)
+  iIntros (Φ) "Hpre HΦ". iDestruct "Hpre" as "%".
+  wp_call. iModIntro.
+  iApply "HΦ".
+  iPureIntro.
+  rewrite clearBit_pure //. word.
+Qed.
+
+End proof.
